src/3d/Translate.fst
@@ -108,6 +108,10 @@ let pk_list = T.({
   pk_kind = PK_list;
   pk_nz = false
 })
+let pk_t_at_most = T.({
+  pk_kind = PK_t_at_most;
+  pk_nz = false
+})
 let pk_filter k = T.({
   pk_kind = PK_filter k;
   pk_nz = k.pk_nz
@@ -286,6 +290,12 @@ let rec parse_typ (env:global_env) (name: A.ident) (t:T.typ) : ML T.parser =
               t
               (T.Parse_nlist e pt)
 
+  | T.T_app {v="t_at_most"} [Inr e; Inl t] ->
+    let pt = parse_typ env name t in
+    mk_parser pk_t_at_most
+              t
+              (T.Parse_t_at_most e pt)
+
   | T.T_app hd args ->
     mk_parser (pk_base hd (parser_kind_nz env hd)) t (T.Parse_app hd args)
 
@@ -436,6 +446,7 @@ let rec parser_is_constant_size_without_actions
       if parser_is_constant_size_without_actions env parse_key
       then parser_is_constant_size_without_actions env parse_value
       else false
+  | T.Parse_t_at_most _ _
   | T.Parse_dep_pair_with_action _ _ _
   | T.Parse_dep_pair_with_refinement_and_action _ _ _ _ _ _
   | T.Parse_refinement_with_action _ _ _ _
@@ -467,6 +478,9 @@ let rec make_validator (env:global_env) (p:T.parser) : ML T.validator =
     else
       pv false p (Validate_nlist n (make_validator env p))
 
+  | Parse_t_at_most n p ->
+    pv false p (Validate_t_at_most n (make_validator env p))  
+    
   | Parse_return e ->
     pv true p Validate_return
 
