src/3d/prelude/Actions.fsti
@@ -278,6 +278,11 @@ val validate_nlist_constant_size_without_actions
   (v: validate_with_action_t p inv l allow_reading)
 : Tot (validate_with_action_t (parse_nlist n p) inv l false)
 
+noextract inline_for_extraction
+val validate_t_at_most (n:U32.t) (#k:parser_kind true) (#t:_) (#p:parser k t)
+                       (#inv:_) (#l:_) (#ar:_) (v:validate_with_action_t p inv l ar)
+  : Tot (validate_with_action_t (parse_t_at_most n p) inv l false)
+
 inline_for_extraction noextract
 val validate_with_comment (c:string)
                           (#nz:_) (#k:parser_kind nz) (#t:_) (#p:parser k t)
